Logical_Equivalence.thy
@@ -9,8 +9,8 @@ text \<open>The definition of formulas is parametric in the index type, but from
 with a fixed (sufficiently large) index type.\<close>
 
 locale indexed_nominal_ts = nominal_ts satisfies transition
-  for satisfies :: "'state\<Colon>fs \<Rightarrow> 'pred\<Colon>fs \<Rightarrow> bool" (infix "\<turnstile>" 70)
-  and transition :: "'state \<Rightarrow> ('act\<Colon>bn,'state) residual \<Rightarrow> bool" (infix "\<rightarrow>" 70) +
+  for satisfies :: "'state::fs \<Rightarrow> 'pred::fs \<Rightarrow> bool" (infix "\<turnstile>" 70)
+  and transition :: "'state \<Rightarrow> ('act::bn,'state) residual \<Rightarrow> bool" (infix "\<rightarrow>" 70) +
   assumes card_idx_perm: "|UNIV::perm set| <o |UNIV::'idx set|"
       and card_idx_state: "|UNIV::'state set| <o |UNIV::'idx set|"
 begin
