README.md
@@ -9,15 +9,15 @@ by Joachim Parrow, Johannes Borgström, Lars-Henrik Eriksson,
 Ram&#363;nas Gutkovas, and Tjark Weber.
 
 These theories are known to work with
-[Isabelle2015](https://isabelle.in.tum.de/)
-and the corresponding version of
-[Nominal2](https://isabelle.in.tum.de/nominal/download.html).
+[Isabelle2016](https://isabelle.in.tum.de/) and the corresponding
+version of Nominal2 from the 2016 release of the [Archive of Formal
+Proofs](http://afp.sourceforge.net/download.shtml).
 
-Assuming both Isabelle2015 and Nominal2 are installed, the theories
+Assuming both Isabelle2016 and Nominal2 are installed, the theories
 may be processed as usual: for instance, in batch mode by executing
 
-  `/path/to/Isabelle2015/bin/isabelle build -d /path/to/Nominal2/ -D .`
+  `/path/to/Isabelle2016/bin/isabelle build -d /path/to/afp-2016-03-02/thys/Nominal2/ -D .`
 
 or interactively in Isabelle/jEdit by executing, e.g.,
 
-  `/path/to/Isabelle2015/bin/isabelle jedit -d /path/to/Nominal2/ -l Nominal2 Equivalence_Implies_Bisimilarity.thy`
+  `/path/to/Isabelle2016/bin/isabelle jedit -d /path/to/afp-2016-03-02/thys/Nominal2/ -l Nominal2 Equivalence_Implies_Bisimilarity.thy`
